ArkLib.lean
@@ -89,6 +89,7 @@ import ArkLib.Interaction.Basic.Decoration
 import ArkLib.Interaction.Basic.MonadDecoration
 import ArkLib.Interaction.Basic.Replicate
 import ArkLib.Interaction.Basic.Syntax
+import ArkLib.Interaction.Basic.Ownership
 import ArkLib.Interaction.Basic.Shape
 import ArkLib.Interaction.Basic.Interaction
 import ArkLib.Interaction.Basic.StateChain
